theories/open.sh
@@ -6,7 +6,7 @@ if [ -f ./settings.sh ]
 then
     source settings.sh
 fi
-COQIDE_OPTIONS="-async-proofs off -async-proofs-command-error-resilience off"
+COQIDE_OPTIONS="-async-proofs off -async-proofs-command-error-resilience off -w -implicits-in-term,-redundant-canonical-projection,-several-object-files,-ambiguous-paths,-implicit-core-hint-db"
 echo "${COQBIN}coqide ${COQIDE_OPTIONS}  `cat _CoqProject` $*"
 ${COQBIN}coqide ${COQIDE_OPTIONS} `cat _CoqProject` $*
 
